theories/interop/wp_prims/readfield.v
@@ -49,8 +49,7 @@ Proof using.
   iApply wp_outcome; first done.
   iApply "Hcont". iFrame.
   iApply ("Cont" with "[- $Hpto]"). iSplit; last done.
-  rewrite /GC /named. iExists _, _, σMLvirt, _. iExists _.
-  iFrame. iPureIntro; split_and!; eauto.
+  rewrite /GC /named. iExists _, _, σMLvirt, _. by iFrame.
 Qed.
 
 End Laws.
